refactor

Spacetalk/VirtualRDA.lean
@@ -1,637 +1,384 @@
-import Spacetalk.HList
-import Spacetalk.Stream
 import Mathlib.Data.Vector
 import Mathlib.Data.List.Range
 import Mathlib.Data.List.Sort
 import Mathlib.Logic.Basic
 import Std.Data.List.Lemmas
-import Mathlib.Tactic.Linarith
+import Mathlib.Data.List.Card
+import Mathlib.Data.Real.Basic
+import Mathlib.Data.Option.Defs
 
-theorem List.mem_pwFilter {l : List α} {R : α → α → Prop} [DecidableRel R] {a : α} : a ∈ l.pwFilter R → a ∈ l := by
-  intro h_mem
-  -- How does the types work here with Set and List?
-  apply Set.mem_of_subset_of_mem (List.pwFilter_subset l (R := R))
-  exact h_mem
+import Spacetalk.HList
+import Spacetalk.Stream
 
--- TODO: Simplify this proof
-theorem List.mem_mergeSort {l : List α} {r : α → α → Prop} [DecidableRel r] {a : α} : a ∈ l.mergeSort r ↔ a ∈ l := by
-  apply Iff.intro
-  · intro h_mem
-    apply Iff.mp
-    apply List.Perm.mem_iff
-    apply List.perm_mergeSort (r := r)
-    exact h_mem
-  · intro h_mem
-    apply Iff.mpr
-    apply List.Perm.mem_iff
-    apply List.perm_mergeSort (r := r)
-    exact h_mem
+inductive Ty
+  | unit
+  | nat
+  | option : Ty → Ty
+deriving BEq, DecidableEq
 
-def finRangeRemovePair (n : Nat) (a b : Fin n) (h : a ≠ b) : Vector (Fin n) (n - 2) :=
-  let v : Vector (Fin n) n := ⟨List.finRange n, List.length_finRange n⟩
-  if h_lt : ↑b < ↑a then
-    let v' := v.removeNth a
-    v'.removeNth ⟨↑b, by
-      apply Nat.lt_of_lt_of_le h_lt
-      apply Nat.le_pred_of_lt
-      exact a.is_lt
-    ⟩
-  else
-    let v' := v.removeNth b
-    v'.removeNth ⟨↑a, by
-      apply Nat.lt_of_lt_of_le
-      · apply Nat.lt_iff_le_and_ne.mpr
-        apply And.intro
-        · exact Nat.not_lt.mp h_lt
-        · apply Fin.val_ne_iff.mpr h
-      · apply Nat.le_pred_of_lt
-        exact b.is_lt
-    ⟩
+@[reducible] def Ty.denote : Ty → Type
+  | unit => Unit
+  | nat => Nat
+  | option ty => Option ty.denote
 
-namespace VirtualRDA
 
-  -- Syntax
+def Ty.default : (ty : Ty) → ty.denote
+  | unit => ()
+  | nat => 0
+  | option _ => none
 
-  inductive Ty
-    | unit
-    | nat
-  deriving BEq, DecidableEq
+theorem Eq.symm_iff : (a = b) ↔ (b = a) := by
+  apply Iff.intro <;> exact Eq.symm
 
-  @[reducible] def Ty.denote : Ty → Type
-    | unit => Unit
-    | nat => Nat
+def Ty.denote_decEq (ty : Ty) (a b : ty.denote) : Decidable (a = b) :=
+  match ty with
+    | .unit => isTrue rfl
+    | .nat => Nat.decEq a b
+    | .option ty' =>
+      match a, b with
+        | none, none => isTrue rfl
+        | none, some _ => isFalse Option.noConfusion
+        | some _, none => isFalse Option.noConfusion
+        | some a', some b' =>
+          match ty'.denote_decEq a' b' with
+            | isTrue h => isTrue (congrArg some h)
+            | isFalse h => isFalse (λ h' => h (Option.some.inj h'))
 
-  instance {ty : Ty} : DecidableEq ty.denote :=
-    λ a b =>
-      match ty with
-        | .unit => isTrue rfl
-        | .nat => Nat.decEq a b
+instance {ty : Ty} : DecidableEq ty.denote :=
+  Ty.denote_decEq ty
 
-  structure TaggedTy (numFifos : Nat) where
-    fid : Fin numFifos
-    ty : Ty
+instance {ty : Ty} : Inhabited ty.denote where
+  default := ty.default
 
-  def TaggedTy.denote {numFifos : Nat} (tty : TaggedTy numFifos) : Type :=
-    tty.ty.denote
+abbrev TyStream (ty : Ty) := Stream' (ty.denote)
 
-  abbrev TaggedHList {numFifos : Nat} (ttys : List (TaggedTy numFifos)) := HList TaggedTy.denote ttys
+abbrev TyStreamsHList (tys : List Ty) := HList TyStream tys
 
-  abbrev TyStream (ty : Ty) := Stream' (ty.denote)
+abbrev TysHList (tys : List Ty) := HList Ty.denote tys
 
-  abbrev TyStreamsHList (tys : List Ty) := HList TyStream tys
+abbrev TysHListStream (tys : List Ty) := Stream' (TysHList tys)
 
-  abbrev TysHList (tys : List Ty) := HList Ty.denote tys
-
-  abbrev TysHListStream (tys : List Ty) := Stream' (TysHList tys)
-
-  def TyStreamsHList.pack (shl : TyStreamsHList tys) : TysHListStream tys :=
-    match tys with
-      | [] => λ _ => []
-      | h::t =>
-        λ n =>
-          let h_elem : h.denote := (shl.get .head) n
-          let tail_streams : TyStreamsHList t :=
-            match shl with
-              | _ :: rest => rest
-          h_elem :: (pack tail_streams) n
-
-  def TysHListStream.unpack (s : TysHListStream tys) : TyStreamsHList tys :=
-    match tys with
-      | [] => []
-      | h::t =>
-        let h_stream : Stream' h.denote := λ n => (s n).get .head
-        let t_stream : TysHListStream t := λ n =>
-          match s n with
+def TyStreamsHList.pack (shl : TyStreamsHList tys) : TysHListStream tys :=
+  match tys with
+    | [] => λ _ => []
+    | h::t =>
+      λ n =>
+        let h_elem : h.denote := (shl.get .head) n
+        let tail_streams : TyStreamsHList t :=
+          match shl with
             | _ :: rest => rest
-        h_stream :: unpack t_stream
+        h_elem :: (pack tail_streams) n
 
-  -- More expressive adds that choose inputs with Fins
-  -- monotonic to preserver old inputs
-  inductive NodeOps : (inputs : List Ty) → List Ty → Type
-    | nop : NodeOps α α -- for stateless nodes
-    | dropAll : NodeOps α []
-    | add : (a : Member .nat inputs) → (b : Member .nat inputs) → NodeOps inputs (.nat :: inputs)
-    | mul : (a : Member .nat inputs) → (b : Member .nat inputs) → NodeOps inputs (.nat :: inputs)
-    | select : (ty : Ty) → (a : Member ty inputs) → NodeOps inputs [ty]
-    | comp : NodeOps α β → NodeOps β γ → NodeOps α γ
+def TysHListStream.unpack (s : TysHListStream tys) : TyStreamsHList tys :=
+  match tys with
+    | [] => []
+    | h::t =>
+      let h_stream : Stream' h.denote := λ n => (s n).get .head
+      let t_stream : TysHListStream t := λ n =>
+        match s n with
+          | _ :: rest => rest
+      h_stream :: unpack t_stream
 
-  structure InputFIFO (inputs : List Ty) (numNodes : Nat) where
-    ty : Ty
-    producer : Member ty inputs
-    consumer : Fin numNodes
-    consumerPort: Nat
-  deriving DecidableEq
+inductive NodeOps : (inputs : List Ty) → List Ty → Type
+  | nop : NodeOps α α -- for stateless nodes
+  | dropAll : NodeOps α []
+  | add : (a : Member .nat inputs) → (b : Member .nat inputs) → NodeOps inputs (.nat :: inputs)
+  | mul : (a : Member .nat inputs) → (b : Member .nat inputs) → NodeOps inputs (.nat :: inputs)
+  | select : (ty : Ty) → (a : Member ty inputs) → NodeOps inputs [ty]
+  | comp : NodeOps α β → NodeOps β γ → NodeOps α γ
 
-  structure OutputFIFO (numNodes : Nat) where
-    ty : Ty
-    producer : Fin numNodes
-    producerPort: Nat
-  deriving DecidableEq
+structure Node where
+  state : List Ty
+  initialState : TysHList state
+  inputs : List Ty
+  outputs : List Ty
+  stateTransform : NodeOps (state ++ inputs) state
+  pipeline : NodeOps (state ++ inputs) outputs
 
-  structure AdvancingFIFO (numNodes : Nat) where
-    ty : Ty
-    producer : Fin numNodes
-    consumer : Fin numNodes
-    producerPort: Nat
-    consumerPort: Nat
-    adv : producer < consumer
-  deriving DecidableEq
+def NodeList (numNodes : Nat) := Vector Node numNodes
 
-  structure InitializedFIFO (numNodes : Nat) where
-    ty : Ty
-    initialValue : ty.denote
-    producer : Fin numNodes
-    consumer : Fin numNodes
-    producerPort: Nat
-    consumerPort: Nat
+structure InputFIFO (inputs : List Ty) (nodes : NodeList numNodes) where
+  ty : Ty
+  producer : Member ty inputs
+  consumer : Fin numNodes
+  consumerPort: Member ty (nodes.get consumer).inputs
+deriving DecidableEq
 
-  instance {nn : Nat} : DecidableEq (InitializedFIFO nn) :=
-    λ a b => by
-      rw [InitializedFIFO.mk.injEq]
-      apply Decidable.byCases (p := a.ty = b.ty)
-      · intro h_ty_eq
-        have h_dety_eq : a.ty.denote = b.ty.denote := by rw [h_ty_eq]
-        apply Decidable.byCases (p := cast h_dety_eq a.initialValue = b.initialValue)
-        · intro h_init_eq
-          apply Decidable.byCases (p := a.producer = b.producer ∧
-                                        a.consumer = b.consumer ∧
-                                        a.producerPort = b.producerPort ∧
-                                        a.consumerPort = b.consumerPort)
-          · intro h_rest_eq
-            apply isTrue
-            apply And.intro h_ty_eq
-            apply And.intro
-            · exact heq_of_cast_eq h_dety_eq h_init_eq
-            · exact h_rest_eq
-          · intro h_rest_neq
-            apply isFalse
-            intro h_eq
-            apply h_rest_neq
-            exact h_eq.right.right
-        · intro h_init_neq
-          apply isFalse
-          intro h_and
-          apply h_init_neq
-          apply cast_eq_iff_heq.mpr
-          exact h_and.right.left
-      · intro h_ty_neq
-        apply isFalse
-        simp
-        intro
-        contradiction
+structure OutputFIFO (outputs : List Ty) (nodes : NodeList numNodes) where
+  ty : Ty
+  producer : Fin numNodes
+  producerPort: Member ty (nodes.get producer).outputs
+  consumer : Member ty outputs
+deriving DecidableEq
 
-  inductive FIFO (inputs : List Ty) (numNodes : Nat)
-    | input : InputFIFO inputs numNodes → FIFO inputs numNodes
-    | output : OutputFIFO numNodes → FIFO inputs numNodes
-    | advancing : AdvancingFIFO numNodes → FIFO inputs numNodes
-    | initialized : InitializedFIFO numNodes → FIFO inputs numNodes
-  deriving DecidableEq
+structure AdvancingFIFO (nodes : NodeList numNodes) where
+  ty : Ty
+  producer : Fin numNodes
+  consumer : Fin numNodes
+  producerPort: Member ty (nodes.get producer).outputs
+  consumerPort: Member ty (nodes.get consumer).inputs
+  adv : producer < consumer
+deriving DecidableEq
 
-  @[simp] def FIFO.ty : FIFO inputs nn → Ty
-    | .input fifo | .output fifo | .advancing fifo | .initialized fifo => fifo.ty
+structure InitializedFIFO (nodes : NodeList numNodes) where
+  ty : Ty
+  initialValue : ty.denote
+  producer : Fin numNodes
+  consumer : Fin numNodes
+  producerPort: Member ty (nodes.get producer).outputs
+  consumerPort: Member ty (nodes.get consumer).inputs
 
-  @[simp] def FIFO.isInput : FIFO inputs nn → Bool
+def aa : True ∧ True := ⟨trivial, trivial⟩
+
+instance {nn : Nat} {nodes : NodeList nn} : DecidableEq (InitializedFIFO nodes) :=
+  λ a b =>
+    let eq := InitializedFIFO.mk.injEq a.ty a.initialValue a.producer a.consumer a.producerPort a.consumerPort b.ty b.initialValue b.producer b.consumer b.producerPort b.consumerPort
+    if h_ty : a.ty = b.ty then
+      have h_dety_eq := congr rfl h_ty
+      if h_init : cast h_dety_eq a.initialValue = b.initialValue then
+        have h_init_eq := heq_of_cast_eq h_dety_eq h_init
+        if h_p : a.producer = b.producer then
+          have h_ppty_eq := by rw[h_ty, h_p]
+          if h_pp : cast h_ppty_eq a.producerPort = b.producerPort then
+            have h_pp_eq := heq_of_cast_eq h_ppty_eq h_pp
+            if h_c : a.consumer = b.consumer then
+              have h_cpty_eq := by rw[h_ty, h_c]
+              if h_cp : cast h_cpty_eq a.consumerPort = b.consumerPort then
+                have h_cp_eq := heq_of_cast_eq h_cpty_eq h_cp
+                isTrue (eq.mpr ⟨h_ty, h_init_eq, h_p, h_c, h_pp_eq, h_cp_eq⟩)
+              else
+                isFalse (λ h_eq => h_cp (cast_eq_iff_heq.mpr (eq.mp h_eq).right.right.right.right.right))
+            else
+              isFalse (λ h_eq => h_c (eq.mp h_eq).right.right.right.left)
+          else
+            isFalse (λ h_eq => h_pp (cast_eq_iff_heq.mpr (eq.mp h_eq).right.right.right.right.left))
+        else
+          isFalse (λ h_eq => h_p (eq.mp h_eq).right.right.left)
+      else
+        isFalse (λ h_eq => h_init (cast_eq_iff_heq.mpr (eq.mp h_eq).right.left))
+    else
+      isFalse (λ h_eq => h_ty (eq.mp h_eq).left)
+
+inductive FIFO {numNodes : Nat} (inputs outputs : List Ty) (nodes : NodeList numNodes)
+  | input : InputFIFO inputs nodes → FIFO inputs outputs nodes
+  | output : OutputFIFO outputs nodes → FIFO inputs outputs nodes
+  | advancing : AdvancingFIFO nodes → FIFO inputs outputs nodes
+  | initialized : InitializedFIFO nodes → FIFO inputs outputs nodes
+deriving DecidableEq
+
+namespace FIFO
+
+  @[simp] def ty : (fifo : FIFO inputs outputs nodes) → Ty
+    | .input f | .output f | .advancing f | .initialized f => f.ty
+
+  @[simp] def isInput : (fifo : FIFO inputs outputs nodes) → Bool
     | .input _ => true
     | _ => false
 
-  @[simp] def FIFO.isOutput : FIFO inputs nn → Bool
+  @[simp] def isOutput : (fifo : FIFO inputs outputs nodes) → Bool
     | .output _ => true
     | _ => false
 
-  def FIFO.consumer : (fifo : FIFO inputs nn) → ¬fifo.isOutput → Fin nn
-    | .initialized fifo', _ | .advancing fifo', _ | .input fifo', _ => fifo'.consumer
-
-  def FIFO.consumerPort : (fifo : FIFO inputs nn) → ¬fifo.isOutput → Nat
-    | .initialized fifo', _ | .advancing fifo', _ | .input fifo', _ => fifo'.consumerPort
-
-  def FIFO.producer : (fifo : FIFO inputs nn) → ¬fifo.isInput → Fin nn
-    | .initialized fifo', _ | .advancing fifo', _ | .output fifo', _ => fifo'.producer
-
-  def FIFO.producerPort : (fifo : FIFO inputs nn) → ¬fifo.isInput → Nat
-    | .initialized fifo, _ | .advancing fifo, _ | .output fifo, _ => fifo.producerPort
-
-  def ConsumerFIFO (inputs : List Ty) (numNodes : Nat) :=
-    {fifo : FIFO inputs numNodes // ¬fifo.isOutput}
-
-  def ConsumerFIFO.consumer (fifo : ConsumerFIFO inputs nn) : Fin nn :=
-    fifo.val.consumer fifo.property
-
-  def ConsumerFIFO.consumerPort (fifo : ConsumerFIFO inputs nn) : Nat :=
-    fifo.val.consumerPort fifo.property
-
-  def ProducerFIFO (inputs : List Ty) (numNodes : Nat) :=
-    {fifo : FIFO inputs numNodes // ¬fifo.isInput}
-
-  def ProducerFIFO.producer (fifo : ProducerFIFO inputs nn) : Fin nn :=
-    fifo.val.producer fifo.property
-
-  def ProducerFIFO.producerPort (fifo : ProducerFIFO inputs nn) : Nat :=
-    fifo.val.producerPort fifo.property
-
-  def FIFOList (inputs : List Ty) (numNodes numFIFOs : Nat) :=
-    {v : Vector (FIFO inputs numNodes) numFIFOs // List.Nodup v.toList}
-
-  namespace FIFOList
-
-    def get (fifos: FIFOList ins nn nf) (i : Fin nf) : FIFO ins nn :=
-      fifos.val.get i
-
-    @[simp] def ty (fifos : FIFOList ins nn nf) (i : Fin nf) :=
-      (fifos.get i).ty
-
-    @[simp] def isNodeInput (fifos : FIFOList ins nn nf) (nid : Fin nn) (i : Fin nf) : Bool :=
-      match fifos.get i with
-        | .input fifo | .advancing fifo | .initialized fifo => fifo.consumer == nid
-        | _ => false
-
-    @[simp] def isNodeOutput (fifos : FIFOList ins nn nf) (nid : Fin nn) (i : Fin nf) : Bool :=
-      match fifos.get i with
-        | .output fifo | .advancing fifo | .initialized fifo => fifo.producer == nid
-        | _ => false
-
-    -- def NonInputFid (fifos : FIFOList ins nn nf) :=
-    --   {fid : Fin nf // (fifos.get fid).isInput = false}
-
-    -- instance {fifos : FIFOList ins nn nf} : BEq fifos.NonInputFid where
-    --   beq := λ a b => a.val = b.val
-
-    -- instance {fifos : FIFOList ins nn nf} : DecidableEq fifos.NonInputFid :=
-    --   λ a b => by
-    --     apply Decidable.byCases (p := a.val = b.val)
-    --     · intro h_eq
-    --       apply isTrue
-    --       apply Subtype.eq
-    --       exact h_eq
-    --     · intro h_neq
-    --       apply isFalse
-    --       intro h_eq
-    --       apply h_neq
-    --       apply Subtype.coe_inj.mpr
-    --       exact h_eq
-
-    -- instance {fifos : FIFOList ins nn nf} : LawfulBEq fifos.NonInputFid where
-    --   eq_of_beq {a b} h := by
-    --     apply Subtype.eq
-    --     simp [BEq.beq] at h
-    --     exact h
-    --   rfl {a} := by simp [BEq.beq]
-
-    -- instance {fifos : FIFOList ins nn nf} {fid : fifos.NonInputFid} : CoeDep fifos.NonInputFid fid (Fin nf) where
-    --   coe := fid.val
-
-    -- def NonOutputFid (fifos : FIFOList ins nn nf) :=
-    --   {fid : Fin nf // (fifos.get fid).isOutput = false}
-
-    -- instance {fifos : FIFOList ins nn nf} : BEq fifos.NonOutputFid where
-    --   beq := λ a b => a.val = b.val
-
-    -- instance {fifos : FIFOList ins nn nf} : DecidableEq fifos.NonOutputFid :=
-    --   λ a b => by
-    --     apply Decidable.byCases (p := a.val = b.val)
-    --     · intro h_eq
-    --       apply isTrue
-    --       apply Subtype.eq
-    --       exact h_eq
-    --     · intro h_neq
-    --       apply isFalse
-    --       intro h_eq
-    --       apply h_neq
-    --       apply Subtype.coe_inj.mpr
-    --       exact h_eq
-
-    -- instance {fifos : FIFOList ins nn nf} : LawfulBEq fifos.NonOutputFid where
-    --   eq_of_beq {a b} h := by
-    --     apply Subtype.eq
-    --     simp [BEq.beq] at h
-    --     exact h
-    --   rfl {a} := by simp [BEq.beq]
-
-    -- instance {fifos : FIFOList ins nn nf} {fid : fifos.NonOutputFid} : CoeDep fifos.NonOutputFid fid (Fin nf) where
-    --   coe := fid.val
-
-    theorem filtered_input_is_not_output {fifos : FIFOList ins nn nf} {fid : Fin nf}
-      (h : fid ∈ (List.finRange nf).filter (fifos.isNodeInput nid))
-      : ¬(fifos.get fid).isOutput := by
-      simp [List.mem_filter] at h
-      cases h_match : fifos.get fid <;> simp; simp [h_match] at h
-
-    def consumer_port_sort_rel {α : Type} {inputs : List Ty} {numNodes : Nat}
-      (a : α × ConsumerFIFO inputs numNodes) (b : α × ConsumerFIFO inputs numNodes) : Prop :=
-      a.snd.consumerPort < b.snd.consumerPort
-
-    theorem consumer_port_sort_rel_eq {inputs : List Ty} {numNodes : Nat} :
-      ∀ α β : Type, (@consumer_port_sort_rel α inputs numNodes = @consumer_port_sort_rel β inputs numNodes) := by
-      sorry
-
-    instance {α : Type} {inputs : List Ty} {numNodes : Nat} : DecidableRel (@consumer_port_sort_rel α inputs numNodes) :=
-      λ a b => by
-        apply Nat.decLt
-
-    def inputTup {fifos : FIFOList ins nn nf} {nid : Fin nn}
-      (fid : {x : Fin nf // x ∈ (List.finRange nf).filter (fifos.isNodeInput nid)})
-      : Fin nf × ConsumerFIFO ins nn :=
-      (fid.val, ⟨fifos.get fid.val, filtered_input_is_not_output fid.property⟩)
-
-    def nodeInputTups (fifos : FIFOList ins nn nf) (nid : Fin nn) : List (Fin nf × ConsumerFIFO ins nn) :=
-      let finRange := List.finRange nf
-      let outputFids := finRange.filter (fifos.isNodeInput nid)
-      let outputTups := outputFids.attach.map inputTup
-      outputTups.mergeSort consumer_port_sort_rel
-
-    @[simp] def nodeInputFids (fifos : FIFOList ins nn nf) (nid : Fin nn) : List (Fin nf) :=
-      let inputTups := fifos.nodeInputTups nid
-      inputTups.map (·.fst)
-
-    @[simp] def NodeInputTys (fifos : FIFOList ins nn nf) (nid : Fin nn) : List Ty :=
-      let inputTups := fifos.nodeInputTups nid
-      inputTups.map (·.snd.val.ty)
-
-    theorem filtered_output_is_not_input {fifos : FIFOList ins nn nf} {fid : Fin nf}
-      (h : fid ∈ (List.finRange nf).filter (fifos.isNodeOutput nid))
-      : ¬(fifos.get fid).isInput := by
-      simp [List.mem_filter] at h
-      cases h_match : fifos.get fid <;> simp; simp [h_match] at h
-
-    def producer_port_sort_rel {α : Type} {inputs : List Ty} {numNodes : Nat}
-      (a : α × ProducerFIFO inputs numNodes) (b : α × ProducerFIFO inputs numNodes) : Prop :=
-      a.snd.producerPort < b.snd.producerPort
-
-    instance {α : Type} {inputs : List Ty} {numNodes : Nat} : DecidableRel (@producer_port_sort_rel α inputs numNodes) :=
-      λ a b => by
-        apply Nat.decLt
-
-    def outputTup {fifos : FIFOList ins nn nf} {nid : Fin nn}
-      (fid : {x : Fin nf // x ∈ (List.finRange nf).filter (fifos.isNodeOutput nid)})
-      : Fin nf × ProducerFIFO ins nn :=
-      (fid.val, ⟨fifos.get fid.val, filtered_output_is_not_input fid.property⟩)
-
-    def nodeOutputTups (fifos : FIFOList ins nn nf) (nid : Fin nn) : List (Fin nf × ProducerFIFO ins nn) :=
-      let finRange := List.finRange nf
-      let outputFids := finRange.filter (fifos.isNodeOutput nid)
-      let outputTups := outputFids.attach.map outputTup
-      outputTups.mergeSort producer_port_sort_rel
-
-    @[simp] def nodeOutputFids (fifos : FIFOList ins nn nf) (nid : Fin nn) : List (Fin nf) :=
-      let outputTups := fifos.nodeOutputTups nid
-      outputTups.map (·.fst)
-
-    @[simp] def NodeOutputTys (fifos : FIFOList ins nn nf) (nid : Fin nn) : List Ty :=
-      let outputTups := fifos.nodeOutputTups nid
-      outputTups.map (·.snd.val.ty)
-
-    -- theorem mem_NodeOutputFids {fifos : FIFOList ins nn nf} {nid : Fin nn} {fid : Fin nf}
-    --   (h : fifos.get fid = fifo) (h_is_not_input : ¬fifo.isInput)
-    --   (h_prod : fifo.producer h_is_not_input = nid)
-    --   : fid ∈ fifos.NodeOutputFids nid := by
-    --   simp only [FIFOList.NodeOutputFidsPreSort]
-    --   apply List.mem_map.mpr
-    --   exists ⟨fid, by
-    --     apply List.mem_filter.mpr
-    --     apply And.intro
-    --     · simp
-    --     · simp
-    --       rw [h]
-    --       cases h_match : fifo
-    --       simp [h_match] at h_is_not_input
-    --       all_goals simp_rw [h_match] at h_prod
-    --       all_goals rw[←h_prod]
-    --       all_goals simp
-    --   ⟩
-    --   apply And.intro
-    --   · apply List.mem_attach
-    --   · rfl
-
-    -- theorem output_fid_idx_lt_output_tys_length {fifos : FIFOList ins nn nf} {fid : Fin nf} {fifo : FIFO ins nn}
-    --   (h : fifos.get fid = fifo) (h_is_not_input : ¬fifo.isInput)
-    --   : (fifos.NodeOutputFids (fifo.producer h_is_not_input)).indexOf fid
-    --     < (fifos.NodeOutputTys (fifo.producer h_is_not_input)).length := by
-    --   have h_len_eq : (fifos.NodeOutputTys (fifo.producer h_is_not_input)).length = (fifos.NodeOutputFids (fifo.producer h_is_not_input)).length := by
-    --     -- apply List.length_map
-    --     sorry
-    --   rw [h_len_eq]
-    --   simp only [List.indexOf]
-    --   apply List.findIdx_lt_length_of_exists
-    --   · exists fid
-    --     apply And.intro
-    --     · simp only [FIFOList.NodeOutputFids]
-    --       sorry
-
-    --       -- apply List.mem_mergeSort (r := vrda.fifos.producer_port_sort_rel).mpr
-    --       -- apply vrda.fifos.mem_NodeOutputFidsPreSort h h_is_not_input
-    --       -- rfl
-    --     · simp
-
-    -- def getOutputFromFid {fifos : FIFOList ins nn nf} {fid : Fin nf} {fifo : FIFO ins nn}
-    --   (h : fifos.get fid = fifo) (h_is_not_input : ¬fifo.isInput)
-    --   (outputs : TysHList (fifos.NodeOutputTys (fifo.producer h_is_not_input))) : fifo.ty.denote :=
-
-    --   let producerId := fifo.producer h_is_not_input
-    --   let outputFids := fifos.NodeOutputFids producerId
-    --   let outputTys := fifos.NodeOutputTys producerId
-
-    --   let idx : Fin outputTys.length := ⟨outputFids.indexOf fid, output_fid_idx_lt_output_tys_length h h_is_not_input⟩
-    --   let h_eq : Member (outputTys.get idx) outputTys = Member fifo.ty outputTys := by
-    --     have : outputTys.get idx = fifo.ty := by
-
-    --       simp_rw [←h]
-    --     rw [this]
-    --   let mem := h_eq ▸ (outputTys.nth_member idx)
-    --   outputs.get mem
-
-  end FIFOList
-
-  structure Node (fifos : FIFOList inputs num_nodes num_fifos) (nid : Fin num_nodes) where
-    state : List Ty
-    initialState : TysHList state
-    stateTransform : NodeOps (state ++ (fifos.NodeInputTys nid)) state
-    pipeline : NodeOps (state ++ (fifos.NodeInputTys nid)) (fifos.NodeOutputTys nid)
-
-  def NodeList (fifos : FIFOList inputs num_nodes num_fifos) :=
-    (nid : Fin num_nodes) → Node fifos nid
-
-  structure VirtualRDA where
-    inputs : List Ty
-    numNodes : Nat
-    numFifos : Nat
-    fifos : FIFOList inputs numNodes numFifos
-    nodes : NodeList fifos
-
-  -- Semantics
-
-  @[simp] def NodeOps.denote : NodeOps α β → (TysHList α → TysHList β)
-    | .nop => id
-    | .dropAll => λ _ => []
-    | .add a b => λ inputs => ((inputs.get a) + (inputs.get b)) :: inputs
-    | .mul a b => λ inputs => ((inputs.get a) * (inputs.get b)) :: inputs
-    | .select _ a => λ inputs => inputs.get a :: []
-    | .comp f g => g.denote ∘ f.denote
-
-  namespace Node
-
-    def nextState (node : Node fifos nid)
-      (inputs : TysHList (fifos.NodeInputTys nid))
-      (currState : TysHList node.state)
-       : TysHList node.state :=
-      node.stateTransform.denote (currState ++ inputs)
-
-    @[simp] def denote (node : Node fifos nid)
-      (inputs : TysHList (fifos.NodeInputTys nid))
-      (currState : TysHList node.state) : TysHList (fifos.NodeOutputTys nid) :=
-      node.pipeline.denote (currState ++ inputs)
-
-  end Node
-
-  namespace VirtualRDA
-
-    def stateMap (vrda : VirtualRDA) :=
-      (nid : Fin vrda.numNodes) → (TysHList (Fin (vrda.numFifos) × vrda.fifos.NodeOutputTys nid)) × (TysHList (vrda.nodes nid).state)
-
-    theorem filtered_output_is_not_input {vrda : VirtualRDA} {fid : Fin vrda.numFifos}
-      (h_mem : fid ∈ (List.finRange vrda.numFifos).filter (λ i => (vrda.fifos.get i).isOutput))
-      : ¬(vrda.fifos.get fid).isInput := by
-      simp [List.mem_filter] at h_mem
-      cases h_match : vrda.fifos.get fid <;> simp; simp [h_match] at h_mem
-
-    def outputFifos (vrda : VirtualRDA) : List (ProducerFIFO vrda.inputs vrda.numNodes) :=
-      let finRange := List.finRange vrda.numFifos
-      let filtered := finRange.filter (λ i => (vrda.fifos.get i).isOutput)
-      filtered.attach.map (λ ⟨fid, h_mem⟩ => ⟨vrda.fifos.get fid, filtered_output_is_not_input h_mem⟩)
-
-    theorem advancing_fifo_lt {vrda : VirtualRDA} {nid : Fin vrda.numNodes} {fid : Fin vrda.numFifos} {fifo : AdvancingFIFO vrda.numNodes}
-      (h_mem : fid ∈ vrda.fifos.NodeInputFids nid) (h_match : vrda.fifos.get fid = FIFO.advancing fifo)
-      : fifo.producer < nid := by
-      have h_is_input : vrda.fifos.isNodeInput nid fid = true := (List.mem_filter.mp h_mem).right
-      simp [h_match] at h_is_input
-      rw [←h_is_input]
-      exact fifo.adv
-
-    def convert_fifo_ty {vrda : VirtualRDA} {fid : Fin vrda.numFifos}
-                      {fifo : FIFO vrda.inputs vrda.numNodes} (h_match : vrda.fifos.get fid = fifo)
-                      (val : fifo.ty.denote)
-                      : (vrda.fifos.ty fid).denote :=
-      let h_eq : fifo.ty = vrda.fifos.ty fid := by simp [h_match]
-      h_eq ▸ val
-
-    -- This is probably no longer true
-    theorem input_map_attach_eq {vrda : VirtualRDA} {nid : Fin vrda.numNodes}
-      : vrda.fifos.NodeInputTys nid = (vrda.fifos.NodeInputFids nid).attach.map vrda.fifos.ty := by
-      -- rw [List.comp_map vrda.fifos.ty]
-      sorry
-
-    def nth_cycle_state (vrda : VirtualRDA) (inputs : TysHListStream vrda.inputs) (n : Nat)
-                        : vrda.stateMap :=
-      λ nid =>
-        let input_fids : List (Fin vrda.numFifos) := vrda.fifos.NodeInputFids nid
-        let input_vals : TysHList (vrda.fifos.NodeInputTys nid) :=
-          input_map_attach_eq ▸ input_fids.attach.to_hlist (vrda.fifos.get_ty Subtype.val ∘ Subtype.val) (
-            λ ⟨fid, h_mem⟩ =>
-              match h_match : vrda.fifos fid.val, fid.property with
-                | .input fifo, _ =>
-                  let val := (inputs n).get fifo.producer
-                  convert_fifo_ty h_match val
-                | .advancing fifo, _ =>
-                  have := advancing_fifo_lt h_mem h_match
-                  let producer_outputs := (vrda.nth_cycle_state inputs n fifo.producer).fst
-                  let val := extract_fifo_output h_match rfl producer_outputs
-                  convert_fifo_ty h_match val
-                | .initialized fifo, _ =>
-                  let val := match n with
-                    | 0 => fifo.initial_value
-                    | n' + 1 =>
-                      let last_outputs := (vrda.nth_cycle_state inputs n' fifo.producer).fst
-                      extract_fifo_output h_match rfl last_outputs
-                  convert_fifo_ty h_match val
-          )
-        let node := vrda.nodes nid
-        let outputs := node.denote input_vals node.initial_state
-        let next_state := node.next_state input_vals node.initial_state
-        (outputs, next_state)
-        termination_by nth_cycle_state _ _ n nid => (n, nid)
-
-    @[simp] def denote (vrda : VirtualRDA) (inputs : TyStreamsHList vrda.inputs)
-                      : TyStreamsHList (vrda.output_fifos.map (vrda.fifos.get_ty Subtype.val)) :=
-      let packed_inputs := inputs.pack
-      let state_stream := vrda.nth_cycle_state packed_inputs
-      let packed_output_stream : TysHListStream (vrda.output_fifos.map (vrda.fifos.get_ty Subtype.val)) :=
-        λ n =>
-          vrda.output_fifos.to_hlist (vrda.fifos.get_ty Subtype.val) (
-            λ fid =>
-              match h_match : vrda.fifos fid.val, fid.property with
-                | .output fifo, _ =>
-                  let producer_outputs := ((state_stream n) fifo.producer).fst
-                  let val := extract_fifo_output h_match rfl producer_outputs
-                  convert_fifo_ty h_match val
-          )
-      packed_output_stream.unpack
-
-
-  end VirtualRDA
-
-    -- builder functions
-
-  theorem congr_contrapositive {f : α → β} {a b : α} (h : f a ≠ f b) : a ≠ b := by
-    intro h_eq
-    apply h
-    rw [h_eq]
-
-  structure IOConnection (vrda : VirtualRDA) where
-    ty : Ty
-    initial_value : ty.denote
-    in_fid : Fin vrda.num_fifos
-    out_fid : Fin vrda.num_fifos
-    in_fifo : InputFIFO vrda.inputs vrda.num_nodes
-    out_fifo : OutputFIFO vrda.num_nodes
-    h_in : (vrda.fifos in_fid) = FIFO.input in_fifo
-    h_out : (vrda.fifos out_fid) = FIFO.output out_fifo
-
-  namespace IOConnection
-
-    theorem io_fifos_neq (ioc : IOConnection vrda) : ioc.in_fid ≠ ioc.out_fid := by
-      have h_fifo_neq : vrda.fifos ioc.in_fid ≠ vrda.fifos ioc.out_fid := by
-        rw [ioc.h_in, ioc.h_out]
-        simp
-      apply congr_contrapositive h_fifo_neq
-
-  end IOConnection
-
-  def make_backedge (vrda : VirtualRDA) (ioc : IOConnection vrda) : VirtualRDA :=
-    let filtered := finRangeRemovePair vrda.num_fifos ioc.in_fid ioc.out_fid ioc.io_fifos_neq
-    let newFIFO := FIFO.initialized {
-      ty := ioc.ty,
-      initial_value := ioc.initial_value,
-      producer := ioc.out_fifo.producer,
-      consumer := ioc.in_fifo.consumer,
-      producer_port := ioc.out_fifo.producer_port,
-      consumer_port := ioc.in_fifo.consumer_port
-    }
-
-    let fifos' : FIFOList vrda.inputs vrda.num_nodes (vrda.num_fifos - 1) :=
-      λ ⟨idx, h_idx⟩ =>
-        if h_lt : idx < (vrda.num_fifos - 2) then
-          let idx' : Fin vrda.num_fifos := filtered.get ⟨idx, h_lt⟩
-          vrda.fifos idx'
+  theorem outputNotInput {fifo : FIFO inputs outputs nodes} : fifo.isOutput = true → fifo.isInput = false := by
+    intro h
+    cases h_match : fifo <;> repeat (first | simp | simp [h_match] at h)
+
+  theorem inputNotOutput {fifo : FIFO inputs outputs nodes} : fifo.isInput = true → fifo.isOutput = false := by
+    intro h
+    cases h_match : fifo <;> repeat (first | simp | simp [h_match] at h)
+
+  def producer {numNodes : Nat} {nodes : NodeList numNodes} : (fifo : @FIFO numNodes inputs outputs nodes) → fifo.isInput = false → Fin numNodes
+    | .initialized f, _ | .advancing f, _ | .output f, _ => f.producer
+
+  def producerPort {numNodes : Nat} {nodes : NodeList numNodes} :
+    (fifo : @FIFO numNodes inputs outputs nodes) → (h : fifo.isInput = false) → Member fifo.ty (nodes.get (fifo.producer h)).outputs
+    | .initialized f, _ | .advancing f, _ | .output f, _ => f.producerPort
+
+  def consumer {numNodes : Nat} {nodes : NodeList numNodes} : (fifo : @FIFO numNodes inputs outputs nodes) → fifo.isOutput = false → Fin numNodes
+    | .initialized f, _ | .advancing f, _ | .input f, _ => f.consumer
+
+  def consumerPort {numNodes : Nat} {nodes : NodeList numNodes} :
+    (fifo : @FIFO numNodes inputs outputs nodes) → (h : fifo.isOutput = false) → Member fifo.ty (nodes.get (fifo.consumer h)).inputs
+    | .initialized f, _ | .advancing f, _ | .input f, _ => f.consumerPort
+
+end FIFO
+
+structure VirtualRDA where
+  inputs : List Ty
+  outputs : List Ty
+  numNodes : Nat
+  nodes : NodeList numNodes
+  fifos : List (FIFO inputs outputs nodes)
+
+@[simp] def NodeOps.denote : NodeOps α β → (TysHList α → TysHList β)
+  | .nop => id
+  | .dropAll => λ _ => []
+  | .add a b => λ inputs => ((inputs.get a) + (inputs.get b)) :: inputs
+  | .mul a b => λ inputs => ((inputs.get a) * (inputs.get b)) :: inputs
+  | .select _ a => λ inputs => inputs.get a :: []
+  | .comp f g => g.denote ∘ f.denote
+
+namespace Node
+
+  def nextState (node : Node)
+    (inputs : TysHList node.inputs)
+    (currState : TysHList node.state)
+      : TysHList node.state :=
+    node.stateTransform.denote (currState ++ inputs)
+
+  @[simp] def denote (node : Node)
+    (inputs : TysHList node.inputs)
+    (currState : TysHList node.state) : TysHList node.outputs :=
+    node.pipeline.denote (currState ++ inputs)
+
+end Node
+
+namespace VirtualRDA
+
+  def FIFOType (vrda : VirtualRDA) := FIFO vrda.inputs vrda.outputs vrda.nodes
+
+  def isNodeInput (vrda : VirtualRDA) {nid : Fin vrda.numNodes} {ty : Ty}
+    (port : Member ty (vrda.nodes.get nid).inputs) (fifo : vrda.FIFOType) : Bool :=
+    match fifo with
+      | .input fifo' | .initialized fifo' | .advancing fifo' =>
+        if h : fifo'.consumer = nid ∧ fifo'.ty = ty then
+          h.left ▸ h.right ▸ fifo'.consumerPort == port
         else
-          newFIFO
+          false
+      | _ => false
 
-    let nodes' : NodeList fifos' :=
-      λ nid =>
-        let node := vrda.nodes nid
-        have inputs_eq : vrda.fifos.NodeInputTys nid = fifos'.NodeInputTys nid := by
-          sorry
-        have outputs_eq : vrda.fifos.NodeOutputTys nid = fifos'.NodeOutputTys nid := by
-          sorry
-        {
-          state := node.state,
-          initial_state := node.initial_state,
-          state_transform := inputs_eq ▸ node.state_transform,
-          pipeline := inputs_eq ▸ outputs_eq ▸ node.pipeline
-          : Node fifos' nid
-        }
+  def isGlobalOutput (vrda : VirtualRDA) {ty : Ty} (output : Member ty vrda.outputs)
+    (fifo : vrda.FIFOType) : Bool :=
+    match fifo with
+      | .output fifo' =>
+        if h : fifo'.ty = ty then
+          h ▸ fifo'.consumer == output
+        else
+          false
+      | _ => false
 
-    { vrda with
-      num_fifos := vrda.num_fifos - 1,
-      fifos := fifos',
-      nodes := nodes'
-    }
+  def stateMap (vrda : VirtualRDA) :=
+    (nid : Fin vrda.numNodes) → (TysHList (vrda.nodes.get nid).outputs) × (TysHList (vrda.nodes.get nid).state)
+
+  def nthCycleState (vrda : VirtualRDA) (inputs : TysHListStream vrda.inputs) (n : Nat)
+                      : vrda.stateMap :=
+    λ nid =>
+      let node := vrda.nodes.get nid
+      let inputsFinRange := List.finRange node.inputs.length
+      have finRange_map_eq : inputsFinRange.map node.inputs.get = node.inputs := by simp [List.get]
+      let nodeInputs : (TysHList node.inputs) := finRange_map_eq ▸ inputsFinRange.toHList node.inputs.get (
+        λ fin =>
+          let port := node.inputs.nthMember fin
+          let fifoOpt := vrda.fifos.find? (vrda.isNodeInput port)
+          match h_match : fifoOpt with
+            | .some fifo =>
+              have h_is_node_input : vrda.isNodeInput port fifo = true := List.find?_some h_match
+              have h_ty_eq : fifo.ty = node.inputs.get fin := by
+                cases h_fm : fifo <;> simp [h_fm, VirtualRDA.isNodeInput] at h_is_node_input <;>
+                (
+                  rename_i fifo'
+                  have p : fifo'.consumer = nid ∧ fifo'.ty = (vrda.nodes.get nid).inputs.get fin := by
+                    apply (dite_eq_iff.mp h_is_node_input).elim
+                    · intro e
+                      exact e.fst
+                    · intro e
+                      have := e.snd
+                      contradiction
+                  exact p.right
+                )
+              match fifo with
+                | .input fifo' =>
+                  h_ty_eq ▸ (inputs n).get fifo'.producer
+                | .advancing fifo' =>
+                  have : fifo'.producer < nid := by
+                    have : fifo'.consumer = nid := by
+                      simp [VirtualRDA.isNodeInput] at h_is_node_input
+                      have p : fifo'.consumer = nid ∧ fifo'.ty = (vrda.nodes.get nid).inputs.get fin := by
+                        apply (dite_eq_iff.mp h_is_node_input).elim
+                        · intro e
+                          exact e.fst
+                        · intro e
+                          have := e.snd
+                          contradiction
+                      exact p.left
+                    rw [←this]
+                    exact fifo'.adv
+                  let producerOutputs := (vrda.nthCycleState inputs n fifo'.producer).fst
+                  h_ty_eq ▸ producerOutputs.get fifo'.producerPort
+                | .initialized fifo' =>
+                  match n with
+                    | 0 => h_ty_eq ▸ fifo'.initialValue
+                    | n' + 1 =>
+                      let producerOutputs := (vrda.nthCycleState inputs n' fifo'.producer).fst
+                      h_ty_eq ▸ producerOutputs.get fifo'.producerPort
+            | .none =>
+              (node.inputs.get fin).default
+      )
+      let currState : TysHList node.state :=
+        match n with
+         | 0 => node.initialState
+         | n' + 1 => (vrda.nthCycleState inputs n' nid).snd
+      let nodeOutputs := node.denote nodeInputs currState
+      let nextState := node.nextState nodeInputs currState
+      (nodeOutputs, nextState)
+      termination_by nthCycleState _ _ n nid => (n, nid)
+
+  def denote (vrda : VirtualRDA) (inputs : TyStreamsHList vrda.inputs)
+                    : TyStreamsHList (vrda.outputs) :=
+    let packedInputs := inputs.pack
+    let stateStream := vrda.nthCycleState packedInputs
+    let outputsFinRange := List.finRange vrda.outputs.length
+    have finRange_map_eq : outputsFinRange.map vrda.outputs.get = vrda.outputs := by simp [List.get]
+    let packedOutputStream : TysHListStream vrda.outputs :=
+      λ n =>
+        finRange_map_eq ▸ outputsFinRange.toHList vrda.outputs.get (
+          λ fin =>
+            let outputMem := vrda.outputs.nthMember fin
+            let fifoOpt := vrda.fifos.find? (vrda.isGlobalOutput outputMem)
+            match h_some : fifoOpt with
+              | .some fifo =>
+                have h_is_output : vrda.isGlobalOutput outputMem fifo = true := List.find?_some h_some
+                have h_ty_eq : fifo.ty = vrda.outputs.get fin := by
+                  cases h_fm : fifo <;> simp [h_fm, VirtualRDA.isGlobalOutput] at h_is_output
+                  rename_i fifo'
+                  apply (dite_eq_iff.mp h_is_output).elim
+                  · intro e
+                    exact e.fst
+                  · intro e
+                    have := e.snd
+                    contradiction
+                match fifo with
+                  | .output fifo' =>
+                    h_ty_eq ▸ (stateStream n fifo'.producer).fst.get fifo'.producerPort
+              | .none =>
+                (vrda.outputs.get fin).default
+        )
+    packedOutputStream.unpack
+
+  -- How does this change the semantics?
+  def connectFIFOs (vrda : VirtualRDA) (ty : Ty)
+    (pi : Fin vrda.fifos.length) (ci : Fin vrda.fifos.length) (init : ty.denote)
+    : VirtualRDA :=
+    let pf := vrda.fifos.get pi
+    let cf := vrda.fifos.get ci
+    if h : pf.isOutput = true ∧ cf.isInput = true ∧ pf.ty = ty ∧ cf.ty = ty then
+      let trimmedFifos := (vrda.fifos.remove pf).remove cf
+      let h_ni : pf.isInput = false := pf.outputNotInput h.left
+      let h_no : cf.isOutput = false := cf.inputNotOutput h.right.left
+      let initFifo : InitializedFIFO vrda.nodes := {
+        ty := ty,
+        initialValue := init,
+        producer := pf.producer h_ni,
+        consumer := cf.consumer h_no,
+        producerPort := h.right.right.left ▸ pf.producerPort h_ni,
+        consumerPort := h.right.right.right ▸ cf.consumerPort h_no,
+      }
+      let newFifo : vrda.FIFOType := FIFO.initialized initFifo
+      let newFifos := newFifo :: trimmedFifos
+      { vrda with
+        fifos := newFifos
+      }
+    else
+      vrda
 
 end VirtualRDA
